\documentclass[a4paper,12pt]{book}      
\usepackage[utf8]{inputenc} 
\usepackage[T1]{fontenc}
\usepackage{times}
\usepackage{amssymb}
\usepackage{amsthm}
\usepackage[polish]{babel}
\newtheorem{df}{Definicja}
\newtheorem{tw}{Twierdzenie}
\newtheorem*{Dowód}{\textmd{\textit{Dowód}}}
\newtheorem{wns}[tw]{\textmd{\textit{Wniosek}}}
\sloppy
\begin{document}     


$$\int_{-1}^{2}(x^2-2x)dx=\left|\begin{array}{c}
	f(x)=x^2-2x \\
	\int f(x)=\frac{x^3}{3}-x^2+C \\
	F(x)= \frac{x^3}{3}-x^2\\
\end{array}
\right|=\left[ \frac{x^3}{3}-x^2 \right]_{-1}^{2}=$$
=\left(\frac{2^3}{3}-2^2\right)-\left(\frac{(-1)^3}{3}-(-1)^2 \right)=\left(\frac{8}{3}-4\right)-\left(-\frac{1}{3}-1\right)=-\frac{4}{3}+\frac{4}{3}=0\\\\
\end{document}
